Some dabbling with the Join Point invariants

examples/ghc/theories/JoinPointInvariants.v
@@ -5,11 +5,14 @@ Require Import VarSet.
 Require Import BasicTypes.
 
 Require Import Coq.Lists.List.
+Require Import Coq.Bool.Bool.
 Require Import Coq.ZArith.BinInt.
 
-Open Scope Z_scope.
-(*
+Set Bullet Behavior "Strict Subproofs".
 
+Open Scope Z_scope.
+
+(*
 Note [Invariants on join points]
 ~~~~~~~~~~~~~~~~~~~~~~~~~~~~~~~~
 Join points must follow these invariants:
@@ -68,12 +71,12 @@ Inductive JoinPointsValid : CoreExpr -> Z -> VarSet -> Prop :=
     GoodJoinRHS a rhs jps ->
     JoinPointsValid body 0 (extendVarSet jps v) ->     (* Tail-call-position *)
     JoinPointsValid (Let (NonRec v rhs) body) n jps
-  | JPV_LetRec  : forall pairs body n jps, 
+  | JPV_LetRec  : forall pairs body n jps,
     (forall v rhs, In (v,rhs) pairs -> isJoinId v = false) ->
     (forall v rhs, In (v,rhs) pairs -> JoinPointsValid rhs 0 emptyVarSet)  -> (* Non-tail-call position *)
     let jps' := delVarSetList jps (map fst pairs) in
     JoinPointsValid body 0 jps' ->     (* Tail-call-position *)
-    JoinPointsValid (Let (Rec pairs) body) n jps'
+    JoinPointsValid (Let (Rec pairs) body) n jps
   | JPV_LetRecJP  : forall pairs body n jps, 
     (forall v rhs, In (v,rhs) pairs -> isJoinId v = true) ->
     let jps' := extendVarSetList jps (map fst pairs) in
@@ -81,14 +84,14 @@ Inductive JoinPointsValid : CoreExpr -> Z -> VarSet -> Prop :=
                      isJoinId_maybe v = Some a ->
                      GoodJoinRHS a rhs jps')  -> (* Non-tail-call position *)
     JoinPointsValid body 0 jps' ->     (* Tail-call-position *)
-    JoinPointsValid (Let (Rec pairs) body) n jps'
+    JoinPointsValid (Let (Rec pairs) body) n jps
   | JPV_Case  : forall scrut bndr ty alts n jps, 
     JoinPointsValid scrut 0 emptyVarSet -> (* Non-tail-call position *)
     let jps' := delVarSet jps bndr in
     (forall dc pats rhs, In (dc,pats,rhs) alts ->
                          let jps' := delVarSetList jps pats in
                          JoinPointsValid rhs 0 jps')  -> (* Tail-call position *)
-    JoinPointsValid (Case scrut bndr ty alts) n jps'
+    JoinPointsValid (Case scrut bndr ty alts) n jps
   | JPV_Cast  : forall e co n jps, 
     JoinPointsValid e 0 jps ->
     JoinPointsValid (Cast e co) n jps
@@ -113,6 +116,15 @@ Inductive JoinPointsValid : CoreExpr -> Z -> VarSet -> Prop :=
 
 (* Attempt two: An executable checker *)
 Fixpoint isJoinPointsValid (e : CoreExpr) (n : Z) (jps : VarSet) {struct e} : bool :=
+  let isJoinPointsValidPair (v : CoreBndr) (rhs : CoreExpr) (jps : VarSet) : bool :=
+    match isJoinId_maybe v with
+    | None => isJoinPointsValid rhs 0 emptyVarSet  (* Non-tail-call position *)
+    | Some a => 
+      if a =? 0 (* Uh, all for the termination checker *)
+      then isJoinPointsValid rhs 0 jps (* tail-call position *)
+      else isJoinRHS a rhs jps                   (* tail-call position *)
+    end
+  in
   match e with
   | Var v => match isJoinId_maybe v with
     | None => true
@@ -124,10 +136,20 @@ Fixpoint isJoinPointsValid (e : CoreExpr) (n : Z) (jps : VarSet) {struct e} : bo
     isJoinPointsValid e2 0 emptyVarSet    (* Non-tail-call position *)
   | Lam v e =>
     isJoinPointsValid e 0 emptyVarSet     (* Non-tail-call position *)
-  | Let bind body => 
-    isJoinPointsValidBind bind jps &&
-    let jps' := delVarSetList jps (bindersOf bind) in
-    isJoinPointsValid body 0 jps'         (* Tail-call-position *)
+  | Let (NonRec v rhs) body => 
+      isJoinPointsValidPair v rhs jps &&
+      let jps' := if isJoinId v
+                  then extendVarSet jps v
+                  else delVarSet    jps v in
+      isJoinPointsValid body 0 jps'
+  | Let (Rec pairs) body => 
+      (forallb (fun p => negb (isJoinId (fst p))) pairs ||
+       forallb (fun p =>       isJoinId (fst p))  pairs) &&
+      let jps' := if forallb (fun p => isJoinId (fst p)) pairs 
+                  then extendVarSetList jps (map fst pairs)
+                  else delVarSetList    jps (map fst pairs) in
+      forallb (fun '(v,e) => isJoinPointsValidPair v e jps') pairs &&
+      isJoinPointsValid body 0 jps'
   | Case scrut bndr ty alts  => 
     isJoinPointsValid scrut 0 emptyVarSet &&  (* Non-tail-call position *)
     let jps' := delVarSet jps bndr in
@@ -146,24 +168,7 @@ with isJoinRHS (a : JoinArity) (rhs : CoreExpr) (jps : VarSet) {struct rhs} : bo
                  then isJoinPointsValid e 0 jps (* tail-call position *)
                  else isJoinRHS (a-1) e jps
     | _ => false
-    end
-with isJoinPointsValidBind (bind : CoreBind) (jps : VarSet) {struct bind} : bool :=
-  let isJoinPointsValidPair (v : CoreBndr) (rhs : CoreExpr) (jps : VarSet) : bool :=
-    match isJoinId_maybe v with
-    | None => isJoinPointsValid rhs 0 emptyVarSet  (* Non-tail-call position *)
-    | Some a => 
-      if a =? 0 (* Uh, all for the termination checker *)
-      then isJoinPointsValid rhs 0 jps (* tail-call position *)
-      else isJoinRHS a rhs jps                   (* tail-call position *)
-    end
-  in
-  match bind with
-  | NonRec v e => isJoinPointsValidPair v e  jps
-  | Rec pairs =>
-    (forallb (fun '(v,e) => negb (isJoinId v)) pairs || forallb (fun '(v,e) => isJoinId v) pairs) &&
-    let jps' := delVarSetList jps (map fst pairs) in
-    forallb (fun '(v,e) => isJoinPointsValidPair v e jps') pairs
-  end.
+    end.
 
 Definition isJoinPointsValidPair (v : CoreBndr) (rhs : CoreExpr) (jps : VarSet) : bool :=
     match isJoinId_maybe v with
@@ -186,4 +191,86 @@ Definition isJoinPointsValidPair (v : CoreBndr) (rhs : CoreExpr) (jps : VarSet) 
       of the top-level recursive functions. Instead, it is a local let and
       I repeat the defininition later to give it a name.
 *)
-   
+
+
+(* Relating the two definitions (may not be needed or useful) *)
+
+
+Scheme JPV_mut := Induction for JoinPointsValid Sort Prop
+with GJR_mut := Induction for GoodJoinRHS Sort Prop.
+
+Axiom isJoinId_eq : forall v,
+  isJoinId v = match isJoinId_maybe v with | None => false |Some _ => true end.
+
+Axiom delVarList_singleton: forall jps v,
+  delVarSetList jps (v :: nil) = delVarSet jps v.
+
+Axiom extendVarList_singleton: forall jps v,
+  extendVarSetList jps (v :: nil) = extendVarSet jps v.
+
+Lemma bindersOf_cleanup:
+  forall {a b} (pairs : list (a * b)),
+  flat_map (fun '(binder, _) => binder :: nil) pairs = map fst pairs.
+Proof. intros.  induction pairs. reflexivity. destruct a0. simpl. rewrite IHpairs. reflexivity. Qed.
+
+Lemma JoinPointsValid_isJoinPointsValid:
+  forall e n jps,
+  JoinPointsValid e n jps -> isJoinPointsValid e n jps = true.
+Proof.
+  eapply JPV_mut with
+    (P0 := fun a rhs jps _ => 
+      (if a =? 0
+        then isJoinPointsValid rhs 0 jps 
+        else isJoinRHS a rhs jps) = true);
+  intros; simpl;
+  rewrite ?isJoinId_eq in *;
+  rewrite ?orb_true_iff, ?andb_true_iff in *;
+  rewrite ?bindersOf_cleanup.
+  * destruct (isJoinId_maybe v); congruence.
+  * rewrite e, Z.leb_le. assumption.
+  * reflexivity.
+  * split; assumption.
+  * assumption.
+  * destruct (isJoinId_maybe v); inversion_clear e.
+    split; assumption.
+  * rewrite e in *; clear e.
+    split; assumption.
+  * split; only 2: split.
+    - rewrite orb_true_iff. left.
+      rewrite forallb_forall.
+      intros [v rhs] HIn.
+      erewrite e by eassumption.
+      reflexivity.
+    - rewrite forallb_forall.
+      intros [v rhs] HIn.
+      specialize (e _ _ HIn).
+      rewrite isJoinId_eq in e.
+      destruct (isJoinId_maybe v); inversion_clear e.
+      specialize (H _ _ HIn).
+      assumption.
+    - rewrite ?orb_true_iff, ?andb_true_iff in *.
+      admit. (* need to handle pairs = [] separately *)
+      (*
+      replace (forallb (fun p : Var.Var * Expr CoreBndr => isJoinId (fst p)) pairs) with false.
+      assumption.
+      symmetry.
+      *)
+  * assert (forallb (fun p : Var.Var * Expr CoreBndr => isJoinId (fst p)) pairs = true).
+    { rewrite forallb_forall.
+      intros [v rhs] HIn.
+      erewrite e by eassumption.
+      reflexivity. }
+    rewrite H1. clear H1.
+    split; only 2: split.
+    - rewrite orb_true_iff. right.
+      reflexivity.
+    - rewrite forallb_forall.
+      intros [v rhs] HIn.
+      specialize (e _ _ HIn).
+      rewrite isJoinId_eq in e.
+      destruct (isJoinId_maybe v) eqn:HiJI; inversion_clear e.
+      specialize (H _ _ _ HIn HiJI).
+      assumption.
+    - rewrite ?orb_true_iff, ?andb_true_iff in *.
+      assumption.
+Admitted.
